lib/Lib.Buffer.fst
@@ -119,8 +119,37 @@ let memset_generic #a #blen b init len =
 
 #set-options "--max_fuel 0"
 
-(* TODO: no null check here too? *)
 let update_sub #t #a #len dst start n src =
+  match t with
+  | MUT ->
+      let h0 = ST.get () in
+      LowStar.BufferOps.blit_non_null (src <: buffer a)
+        0ul (dst <: buffer a) (size_to_UInt32 start) (size_to_UInt32 n);
+      let h1 = ST.get () in
+      assert (forall (k:nat{k < v n}). bget h1 dst (v start + k) == bget h0 src k);
+      FStar.Seq.lemma_eq_intro
+        (as_seq h1 dst)
+        (Seq.update_sub #a #(v len) (as_seq h0 dst) (v start) (v n) (as_seq h0 src))
+  | IMMUT ->
+      let h0 = ST.get () in
+      LowStar.BufferOps.blit_non_null (src <: ibuffer a)
+        0ul (dst <: buffer a) (size_to_UInt32 start) (size_to_UInt32 n);
+      let h1 = ST.get () in
+      assert (forall (k:nat{k < v n}). bget h1 dst (v start + k) == bget h0 src k);
+      FStar.Seq.lemma_eq_intro
+        (as_seq h1 dst)
+        (Seq.update_sub #a #(v len) (as_seq h0 dst) (v start) (v n) (as_seq h0 src))
+  | CONST ->
+      let h0 = ST.get () in
+      LowStar.BufferOps.blit_non_null (CB.cast (src <: cbuffer a))
+        0ul (dst <: buffer a) (size_to_UInt32 start) (size_to_UInt32 n);
+      let h1 = ST.get () in
+      assert (forall (k:nat{k < v n}). bget h1 dst (v start + k) == bget h0 src k);
+      FStar.Seq.lemma_eq_intro
+        (as_seq h1 dst)
+        (Seq.update_sub #a #(v len) (as_seq h0 dst) (v start) (v n) (as_seq h0 src))
+
+let update_sub_generic #t #a #len dst start n src =
   match t with
   | MUT ->
       let h0 = ST.get () in
@@ -162,19 +191,19 @@ let update_sub_f #a #len h0 buf start n spec f =
 
 let concat2 #a #t0 #t1 len0 s0 len1 s1 s =
   let h0 = ST.get () in
-  update_sub s (size 0) len0 s0;
-  update_sub s len0 len1 s1;
+  update_sub_generic s (size 0) len0 s0;
+  update_sub_generic s len0 len1 s1;
   let h1 = ST.get () in
   Seq.eq_intro (Seq.sub (as_seq h1 s) 0 (v len0)) (as_seq h0 s0);
   Seq.lemma_concat2 (v len0) (as_seq h0 s0) (v len1) (as_seq h0 s1) (as_seq h1 s)
 
 let concat3 #a #t0 #t1 #t2 len0 s0 len1 s1 len2 s2 s =
   let h0 = ST.get () in
-  update_sub s (size 0) len0 s0;
-  update_sub s len0 len1 s1;
+  update_sub_generic s (size 0) len0 s0;
+  update_sub_generic s len0 len1 s1;
   let h1 = ST.get () in
   Seq.eq_intro (Seq.sub (as_seq h1 s) 0 (v len0)) (as_seq h0 s0);
-  update_sub s (len0 +! len1) len2 s2;
+  update_sub_generic s (len0 +! len1) len2 s2;
   let h2 = ST.get () in
   Seq.eq_intro (Seq.sub (as_seq h2 s) 0 (v len0)) (as_seq h0 s0);
   Seq.eq_intro (Seq.sub (as_seq h2 s) (v len0) (v len1)) (as_seq h0 s1);
